Complete characterisation of nullability for sentential forms.

examples/parsing/NTpropertiesScript.sml
@@ -6,17 +6,27 @@ open pred_setTheory
 
 val _ = new_theory "NTproperties"
 
-val dsimp = simp_tac (srw_ss() ++ boolSimps.DNF_ss)
-
-val nullable_def = Define`
-  nullable G sf = derives G sf []
-`
-
+fun dsimp thl = asm_simp_tac (srw_ss() ++ boolSimps.DNF_ss) thl
+fun asimp thl = asm_simp_tac (srw_ss() ++ ARITH_ss) thl
 fun qxchl [] ttac = ttac
   | qxchl (q::qs) ttac = Q.X_CHOOSE_THEN q (qxchl qs ttac)
 
 val APPEND_EQ_SING' = CONV_RULE (LAND_CONV (ONCE_REWRITE_CONV [EQ_SYM_EQ]))
                                 listTheory.APPEND_EQ_SING
+
+val RTC_R_I = relationTheory.RTC_RULES |> SPEC_ALL |> CONJUNCT2 |> GEN_ALL
+
+(* ----------------------------------------------------------------------
+    A sentential form is nullable if it can derive the empty string.
+
+    This work draws on Aditi Barthwal's formalisation.  Using parse trees
+    rather than derivations simplifies some of the resulting proofs.
+   ---------------------------------------------------------------------- *)
+
+val nullable_def = Define`
+  nullable G sf = derives G sf []
+`
+val _ = overload_on ("nullableNT", ``λG n. nullable G [NT n]``)
 
 val derives_TOK = store_thm(
   "derives_TOK",
@@ -44,8 +54,7 @@ val derives_TOK = store_thm(
   ] >>
   simp[] >> disch_then (qxchl [`ps`, `ss`] strip_assume_tac) >>
   map_every qexists_tac [`ps`, `ss`] >> simp[] >>
-  match_mp_tac (CONJUNCT2 (SPEC_ALL relationTheory.RTC_RULES)) >>
-  simp[derive_def] >> metis_tac[])
+  match_mp_tac RTC_R_I >> simp[derive_def] >> metis_tac[])
 
 val nullable_CONS_TOK = store_thm(
   "nullable_CONS_TOK",
@@ -54,7 +63,54 @@ val nullable_CONS_TOK = store_thm(
   qspecl_then [`G`, `[]`, `rest`, `t`, `[]`] mp_tac derives_TOK >> simp[])
 val _ = export_rewrites ["nullable_CONS_TOK"]
 
-val _ = overload_on ("nullableNT", ``λG n. nullable G [NT n]``)
+val nullable_NIL = store_thm(
+  "nullable_NIL",
+  ``nullable G [] = T``,
+  simp[nullable_def])
+val _ = export_rewrites ["nullable_NIL"]
+
+val derives_split_horizontally = store_thm(
+  "derives_split_horizontally",
+  ``∀p s sf. derives G (p ++ s) sf ⇔
+             ∃sf1 sf2. sf = sf1 ++ sf2 ∧ derives G p sf1 ∧ derives G s sf2``,
+  rpt gen_tac >> REVERSE eq_tac >- metis_tac [derives_paste_horizontally] >>
+  `∃sf0. p ++ s = sf0` by simp[] >> simp[] >>
+  pop_assum
+    (fn th => disch_then
+                (fn th2 => mp_tac th >> map_every qid_spec_tac [`s`, `p`] >>
+                           mp_tac th2)) >>
+  map_every qid_spec_tac [`sf`, `sf0`] >>
+  ho_match_mp_tac relationTheory.RTC_INDUCT >> simp[] >> conj_tac
+  >- metis_tac[relationTheory.RTC_REFL] >>
+  map_every qx_gen_tac [`sf0`, `sf'`, `sf`] >> simp[derive_def] >>
+  disch_then (CONJUNCTS_THEN2
+               (qxchl [`pfx`, `N`, `r`, `sfx`] strip_assume_tac)
+               strip_assume_tac) >> rw[] >>
+  qpat_assum `X = Y` mp_tac >> simp[listTheory.APPEND_EQ_APPEND_MID] >>
+  disch_then (DISJ_CASES_THEN (qxchl [`l`] strip_assume_tac)) >> rw[] >|[
+    first_x_assum (qspecl_then [`pfx ++ r ++ l`, `s`] mp_tac),
+    first_x_assum (qspecl_then [`p`, `l ++ r ++ sfx`] mp_tac)
+  ] >> simp[] >> disch_then (qxchl [`sf1`, `sf2`] strip_assume_tac) >> rw[] >>
+  map_every qexists_tac [`sf1`, `sf2`] >> simp[] >> match_mp_tac RTC_R_I >>
+  metis_tac[derive_def]);
+
+val nullable_CONS_NT = store_thm(
+  "nullable_CONS_NT",
+  ``nullable G (NT n :: rest) <=>
+      nullable G rest ∧ n ∈ FDOM G.rules ∧
+      ∃r. r ∈ G.rules ' n ∧ nullable G r``,
+  simp[nullable_def] >> REVERSE eq_tac
+  >- (strip_tac >> match_mp_tac RTC_R_I >> simp[derive_def] >>
+      qexists_tac `r ++ rest` >> REVERSE conj_tac
+      >- metis_tac[derives_paste_horizontally, listTheory.APPEND] >>
+      qexists_tac `[]` >> simp[]) >>
+  `NT n :: rest = [NT n] ++ rest` by simp[] >> pop_assum SUBST1_TAC >>
+  simp[derives_split_horizontally] >> strip_tac >>
+  Q.UNDISCH_THEN `derives G [NT n] []`
+     (mp_tac o SIMP_RULE (srw_ss()) [Once relationTheory.RTC_CASES1]) >>
+  metis_tac[]);
+
+
 
 val paireq = prove(
   ``(x,y) = z ⇔ x = FST z ∧ y = SND z``, Cases_on `z` >> simp[])
@@ -67,12 +123,16 @@ val GSPEC_INTER = prove(
 
 val _ = SIMP_CONV (srw_ss())[GSPEC_INTER, combinTheory.o_ABS_R, combinTheory.S_ABS_R, combinTheory.S_ABS_L, pairTheory.o_UNCURRY_R, pairTheory.S_UNCURRY_R] ``{ n + m | n > 10 ∧ m < 3 } ∩ Q``
 
+(* nullableML is an "executable" version of nullable that examines the grammar
+   to determine nullability. I put the "executable" in quotes because of the
+   scary looking set comprehension below.  This will work fine if the
+   sets of rules for non-terminals are always finite. *)
 val nullableML_def = tDefine "nullableML" `
   nullableML seen [] = T ∧
   nullableML seen (TOK t :: _) = F ∧
   nullableML seen (NT n :: rest) =
       if n ∈ FDOM G.rules ∧ n ∉ seen then
-        if G.rules ' n ∩ nullableML (n INSERT seen) = ∅ then F
+        if G.rules ' n ∩ { r | nullableML (n INSERT seen) r } = ∅ then F
         else nullableML seen rest
       else F
 `
@@ -88,14 +148,109 @@ val nullableML_def = tDefine "nullableML" `
    pop_assum (MATCH_MP_TAC o MATCH_MP CARD_SUBSET) >>
    simp[SUBSET_DEF])
 
-(*
+val nullableML_nullable = store_thm(
+  "nullableML_nullable",
+  ``∀sn sf. nullableML G sn sf ⇒ nullable G sf``,
+  HO_MATCH_MP_TAC (theorem "nullableML_ind") >>
+  simp[nullableML_def, nullable_CONS_NT] >>
+  map_every qx_gen_tac [`sn`, `N`, `sf`] >> rpt strip_tac >>
+  qpat_assum `SS ≠ ∅` mp_tac >> simp[EXTENSION] >> metis_tac[]);
+
+
+val ptree_NTs_def = tDefine "ptree_NTs" `
+  (ptree_NTs (Lf l) = case l of NT N => {N} | _ => ∅) ∧
+  (ptree_NTs (Nd n subs) = n INSERT BIGUNION (IMAGE ptree_NTs (set subs)))
+`
+  (WF_REL_TAC `measure ptree_size` >> Induct_on `subs` >> simp[] >> fs[] >>
+   rpt strip_tac >> res_tac >> asimp[])
+
+val ptree_rptfree_def = tDefine "ptree_rptfree" `
+  ptree_rptfree (Lf _) = T ∧
+  ptree_rptfree (Nd N subs) =
+    ∀s. MEM s subs ⇒ ptree_rptfree s ∧ N ∉ ptree_NTs s
+`
+  (WF_REL_TAC `measure ptree_size` >> Induct_on `subs` >> simp[] >> fs[] >>
+   rpt strip_tac >> res_tac >> asimp[])
+
+val nullableML_by_singletons = store_thm(
+  "nullableML_by_singletons",
+  ``nullableML G sn sf ⇔ ∀a. MEM a sf ⇒ nullableML G sn [a]``,
+  Induct_on `sf` >> dsimp[nullableML_def] >> qx_gen_tac `h` >>
+  Cases_on `h` >> simp[nullableML_def, CONJ_ASSOC]);
+
+val nullable_by_singletons = store_thm(
+  "nullable_by_singletons",
+  ``nullable G sf ⇔ ∀a. MEM a sf ⇒ nullable G [a]``,
+  Induct_on `sf` >> simp[] >> qx_gen_tac `h` >> Cases_on `h` >>
+  dsimp[nullable_CONS_NT] >> metis_tac[])
+
+val ptree_nullableML = store_thm(
+  "ptree_nullableML",
+  ``∀pt sn. DISJOINT (ptree_NTs pt) sn ∧ ptree_fringe pt = [] ∧
+            valid_ptree G pt ∧ ptree_rptfree pt ⇒
+            nullableML G sn [ptree_head pt]``,
+  HO_MATCH_MP_TAC grammarTheory.ptree_ind >>
+  simp[nullableML_def, ptree_NTs_def, ptree_rptfree_def] >>
+  qx_gen_tac `subs` >> strip_tac >> dsimp[] >>
+  dsimp[FLAT_EQ_NIL, listTheory.MEM_MAP] >> map_every qx_gen_tac [`N`, `sn`] >>
+  strip_tac >> simp[EXTENSION] >> qexists_tac `MAP ptree_head subs` >> simp[] >>
+  simp[Once nullableML_by_singletons] >> dsimp[listTheory.MEM_MAP] >>
+  `∀p. MEM p subs ⇒ DISJOINT (ptree_NTs p) (N INSERT sn)`
+    suffices_by simp[] >>
+  simp[Once DISJOINT_SYM, DISJOINT_INSERT] >> simp[Once DISJOINT_SYM]);
+
+val rptfree_subtree = store_thm(
+  "rptfree_subtree",
+  ``∀pt. ptree_rptfree pt ∧ N ∈ ptree_NTs pt ∧ ptree_fringe pt = [] ∧
+         valid_ptree G pt ⇒
+         ∃pt'. ptree_rptfree pt' ∧ ptree_head pt' = NT N ∧
+               ptree_fringe pt' = [] ∧ valid_ptree G pt'``,
+  HO_MATCH_MP_TAC grammarTheory.ptree_ind >>
+  simp[ptree_rptfree_def, ptree_NTs_def] >> qx_gen_tac `subs` >> strip_tac >>
+  dsimp[listTheory.MEM_MAP, FLAT_EQ_NIL] >> conj_tac
+  >- (strip_tac >> qexists_tac `Nd N subs` >>
+      dsimp[ptree_rptfree_def, FLAT_EQ_NIL, listTheory.MEM_MAP]) >>
+  map_every qx_gen_tac [`N'`, `pt`] >> strip_tac >> metis_tac[]);
+
+val rptfree_nullable_ptrees_possible = store_thm(
+  "rptfree_nullable_ptrees_possible",
+  ``∀pt. valid_ptree G pt ∧ ptree_fringe pt = [] ⇒
+         ∃pt'. valid_ptree G pt' ∧ ptree_head pt' = ptree_head pt ∧
+               ptree_fringe pt' = [] ∧ ptree_rptfree pt'``,
+  HO_MATCH_MP_TAC grammarTheory.ptree_ind >>
+  dsimp[FLAT_EQ_NIL, listTheory.MEM_MAP] >>
+  map_every qx_gen_tac [`subs`, `N`] >> rpt strip_tac >>
+  `∃subs'. MAP ptree_head subs' = MAP ptree_head subs ∧
+           ∀p. MEM p subs' ⇒
+                 valid_ptree G p ∧ ptree_fringe p = [] ∧
+                 ptree_rptfree p`
+    by (qpat_assum `MAP ptree_head subs ∈ G.rules ' N` (K ALL_TAC) >>
+        Induct_on `subs` >- (rpt strip_tac >> qexists_tac `[]` >> simp[]) >>
+        dsimp[] >> qx_gen_tac `h` >> rpt strip_tac >> fs[] >>
+        qexists_tac `pt'::subs'` >> dsimp[]) >>
+  Cases_on `∃pt. MEM pt subs' ∧ N ∈ ptree_NTs pt`
+  >- (fs[] >> metis_tac[rptfree_subtree]) >>
+  fs[] >> qexists_tac `Nd N subs'` >>
+  dsimp[ptree_rptfree_def, FLAT_EQ_NIL, listTheory.MEM_MAP] >> metis_tac[])
+
 val nullable_nullableML = store_thm(
   "nullable_nullableML",
-  ``∀sn sf. nullable G sf ∧ (∀n. n ∈ sn ⇒ ¬nullable G [NT n]) ⇒
-            nullableML G sn sf``,
-  HO_MATCH_MP_TAC (theorem "nullableML_ind") >> simp[nullableML_def] >>
-  rpt strip_tac
+  ``∀sf. nullable G sf ⇒ nullableML G ∅ sf``,
+  simp[Once nullable_by_singletons, Once nullableML_by_singletons] >>
+  ntac 2 strip_tac >> qx_gen_tac `a` >> strip_tac >>
+  `nullable G [a]` by res_tac >>
+  `derives G [a] []` by fs[nullable_def] >>
+  qspecl_then [`Lf a`, `[]`] mp_tac ptrees_derive_extensible >> simp[] >>
+  disch_then (qxchl [`pt`] strip_assume_tac) >>
+  `∃pt'. ptree_rptfree pt' ∧ ptree_head pt' = ptree_head pt ∧
+         ptree_fringe pt' = [] ∧ valid_ptree G pt'`
+    by metis_tac [rptfree_nullable_ptrees_possible] >>
+  qspecl_then [`pt'`, `∅`] mp_tac ptree_nullableML >> simp[]);
 
-*)
+val nullableML_EQN = store_thm(
+  "nullableML_EQN",
+  ``nullable G sf ⇔ nullableML G ∅ sf``,
+  metis_tac[nullable_nullableML, nullableML_nullable])
+
 
 val _ = export_theory()
